Diff/RobustSSCHCriterion.v
@@ -1,0 +1,124 @@
+From mathcomp Require Import all_ssreflect.
+
+Set Implicit Arguments.
+Unset Printing Implicit Defensive.
+
+Require Import ClassicalExtras.
+Require Import MyNotation.
+Require Import Setoid.
+Require Import FunctionalExtensionality.
+Require Import Setoid.
+
+Require Import Galois.
+Require Import LanguageModel.
+Require Import TraceModel.
+Require Import Properties.
+Require Import ChainModel.
+Require Import RobustSSCHPreservation.
+
+Hypothesis prop_extensionality : forall A B : Prop, (A <-> B) -> A = B.
+
+Section RobustSSCHCriterion.
+
+  Variable Source Target: Language.
+  Variable compilation_chain : CompilationChain Source Target.
+
+  (*CA: we don't need a particular structure of traces to define preservation
+        e.g. traces = values or our defn of traces both make sense
+   *)
+  Variable trace__S trace__T : Set.
+
+  Local Definition prop__S := prop trace__S.
+  Local Definition prop__T := prop trace__T.
+  Local Definition hprop__S := hprop trace__S.
+  Local Definition hprop__T := hprop trace__T.
+
+  
+  Variable Source_Semantics : Semantics Source trace__S.
+  Variable Target_Semantics : Semantics Target trace__T.
+
+  Local Definition sem__S := sem Source_Semantics.
+  Local Definition sem__T := sem Target_Semantics.
+  Local Definition beh__S := beh Source_Semantics.
+  Local Definition beh__T := beh Target_Semantics. 
+  Local Definition par__S := par Source.
+  Local Definition par__T := par Target.
+  Local Definition ctx__S := ctx Source.
+  Local Definition ctx__T := ctx Target. 
+  Local Definition rhsat__S := rhsat Source_Semantics.
+  Local Definition rhsat__T := rhsat Target_Semantics.
+  
+  Local Definition cmp := compile_par Source Target compilation_chain.
+
+  Local Notation "P ↓" := (cmp P) (at level 50).
+
+  Local Definition plug__S:= plug Source.
+  Local Definition plug__T := plug Target.
+  
+  Variable rel : trace__S -> trace__T -> Prop.
+
+  Local Definition adjunction :=  induced_connection rel.
+
+  Local Definition τ' : prop__S -> prop__T := α adjunction.
+  Local Definition σ' : prop__T -> prop__S := γ adjunction.
+
+  Local Definition rel_adjunction_law : Adjunction_law τ' σ' := adjunction_law adjunction.
+
+  Definition rel_RSCHC := forall P C__T, exists C__S,
+       ( forall t, sem__T (plug__T (P ↓) C__T) t -> exists s, rel s t /\ sem__S (plug__S P C__S) s).
+
+  Local Definition sCl_σ : hprop__T -> hprop__S := sCl_σ σ'.
+  Local Definition sCl_τ : hprop__S -> hprop__T := sCl_τ τ'. 
+  
+  Local Definition sCl_τRhP := sCl_τRhP compilation_chain
+                                        Source_Semantics Target_Semantics
+                                        τ'.
+
+
+  Local Definition sCl_σRhP := sCl_σRhP compilation_chain
+                                        Source_Semantics Target_Semantics
+                                        σ'.
+
+
+  Lemma sCl_σRhP_sCl_τRhP : (forall (P : par__S) (H__T : hprop__T), SSC H__T ->  sCl_σRhP P H__T) <->
+                            (forall (P : par__S) (H__S : hprop__S), SSC H__S -> sCl_τRhP P H__S).
+  Proof.         
+    split.
+    + move => Hσ P H__S ssc_H rsat_source. 
+      have rsat_sigma_tau : rhsat__S P (sCl_σ (sCl_τ H__S)).  
+      { apply: rhsat_upper_closed. exact rsat_source.
+        apply: Galois_snd_lift. exact rel_adjunction_law. exact ssc_H. }       
+      have τ_ssc : SSC (sCl_τ H__S) by apply: sCl_SCH.
+      exact (Hσ P (sCl_τ H__S) τ_ssc rsat_sigma_tau).  
+    + move => Hτ P H__T ssc_H rsat_source.
+      have h_ssc: SSC (sCl_σ H__T) by apply: sCl_SCH.
+      move: (Hτ P (sCl_σ H__T) h_ssc rsat_source).
+      move => HHH. eapply rhsat_upper_closed. exact HHH.
+      apply: Galois_fst_lift; eauto. exact rel_adjunction_law. 
+  Qed.
+
+  Theorem rel_RSCHC_sClτRSCHP : rel_RSCHC <-> (forall (P : par__S) (H__S : hprop__S), SSC H__S -> sCl_τRhP P H__S).
+  Proof.
+    split. 
+    - move => Htilde P H H_ssc. setoid_rewrite contra_τRhP.
+      move => [C__T Hsem].  
+      move: (Htilde P C__T) => [C__S HH]. exists C__S => Hfalse.
+      apply: Hsem. 
+      exists (τ' (beh__S (plug__S P C__S))). split.
+      + by exists (beh__S (plug__S P C__S)). 
+      + move => t Ht. destruct (HH t Ht) as [s [Hs1 Hs2]]. now exists s.
+    - move => Hτ P Ct.
+      have Hssc : SSC (fun b: prop__S =>  ~ beh__T (plug__T (P↓) Ct) ⊆ τ' b).
+      { move => b1 Hb1 b2 b1_b2 Hb2. apply: Hb1. firstorder. }    
+      specialize (Hτ P (fun b: prop__S =>  ~ beh__T (plug__T (P↓) Ct) ⊆ τ' b) Hssc).
+      apply contra in Hτ. move: Hτ. rewrite !neg_rhsat. 
+      move => [Cs Hbeh]. move/NNPP: Hbeh. 
+      exists Cs => t Hsem_t. move: (Hbeh t Hsem_t). firstorder.
+      move => Hf. specialize (Hf Ct).
+      destruct Hf as [b' [Hb' Hbb]]. destruct Hb' as [bs [Hbs1 Hbs2]]. now subst.  
+  Qed.    
+
+  Theorem rel_RTC_σRTP : rel_RSCHC <-> (forall (P : par__S) (H__T : hprop__T), SSC H__T ->  sCl_σRhP P H__T).
+  Proof. by rewrite sCl_σRhP_sCl_τRhP rel_RSCHC_sClτRSCHP. Qed.
+
+End RobustSSCHCriterion.
